run_default, start of run_code

CoqOfRust/revm/links/dependencies.v
@@ -3,6 +3,7 @@ Require Import CoqOfRust.links.M.
 Require Import core.convert.links.mod.
 Require Import core.links.array.
 Require core.links.clone.
+Require core.links.default.
 Import Run.
 
 Module ruint.
@@ -211,6 +212,31 @@ Module alloy_primitives.
           }
         Defined.
       End Impl_Clone_for_Bytes.
+
+      Module Impl_Default_for_Bytes.
+        Definition Self : Ty.t := Ty.path "alloy_primitives::bytes_::Bytes".
+
+        Parameter default : PolymorphicFunction.t.
+
+        Axiom Implements :
+          M.IsTraitInstance
+            "default::default::Default"
+            (* Trait polymorphic consts *) []
+            (* Trait polymorphic types *) []
+            Self
+            (* Instance *) [ ("default", InstanceField.Method default) ].
+
+        Definition run_default : default.Default.Run_default Bytes.t.
+        Admitted.
+      
+        Definition run : default.Default.Run Bytes.t.
+        Proof.
+          constructor.
+          { (* clone *)
+            exact run_default.
+          }
+        Defined.
+      End Impl_Default_for_Bytes.
     End bytes_.
   End links.
 End alloy_primitives.
